tactics

MathematicalLogic/Equality/Rewrite.lean
@@ -3,86 +3,61 @@ import MathematicalLogic.Equality.Theory
 variable [EqLanguage 𝓛] {𝓣 : Theory 𝓛} [EqTheory 𝓣]
 
 mutual
-inductive Term.Rewritable (t₁ t₂ : Term 𝓛) : Term 𝓛 → Term 𝓛 → Prop where
-| matched : Term.Rewritable t₁ t₂ t₁ t₂
-| func {ts₁ ts₂ : Terms 𝓛 n} :
-  Terms.Rewritable t₁ t₂ ts₁ ts₂ → Term.Rewritable t₁ t₂ (f ⬝ₜ ts₁) (f ⬝ₜ ts₂)
-| refl : Term.Rewritable t₁ t₂ t t
-inductive Terms.Rewritable (t₁ t₂ : Term 𝓛) : Terms 𝓛 n → Terms 𝓛 n → Prop where
-| nil : Terms.Rewritable t₁ t₂ []ₜ []ₜ
-| cons :
-  Term.Rewritable t₁ t₂ t₁' t₂' → Terms.Rewritable t₁ t₂ ts₁ ts₂ →
-  Terms.Rewritable t₁ t₂ (t₁' ∷ₜ ts₁) (t₂' ∷ₜ ts₂)
+inductive Term.Rewritable (Γ : Context 𝓛) : Term 𝓛 → Term 𝓛 → Prop where
+| matched : Γ ⊢ t₁ ≈ t₂ → Term.Rewritable Γ t₁ t₂
+| func : Terms.Rewritable Γ ts₁ ts₂ → Term.Rewritable Γ (f ⬝ₜ ts₁) (f ⬝ₜ ts₂)
+| refl : Term.Rewritable Γ t t
+inductive Terms.Rewritable (Γ : Context 𝓛) : Terms 𝓛 n → Terms 𝓛 n → Prop where
+| nil : Terms.Rewritable Γ []ₜ []ₜ
+| cons : Term.Rewritable Γ t₁ t₂ → Terms.Rewritable Γ ts₁ ts₂ →
+  Terms.Rewritable Γ (t₁ ∷ₜ ts₁) (t₂ ∷ₜ ts₂)
 end
 
-inductive Formula.Rewritable (t₁ t₂ : Term 𝓛) : Formula 𝓛 → Formula 𝓛 → Prop where
-| atom : Terms.Rewritable t₁ t₂ ts₁ ts₂ → Formula.Rewritable t₁ t₂ (p ⬝ₚ ts₁) (p ⬝ₚ ts₂)
-| fal : Formula.Rewritable t₁ t₂ ⊥ ⊥
-| imp :
-  Formula.Rewritable t₁ t₂ p₁ p₂ → Formula.Rewritable t₁ t₂ q₁ q₂ →
-  Formula.Rewritable t₁ t₂ (p₁ ⟶ q₁) (p₂ ⟶ q₂)
-| all : Formula.Rewritable t₁ t₂ (∀' p) (∀' p)
-
--- namespace Formula.Rewritable
-
--- def eq : Term.Rewritable t₁ t₂ t₁' t₂' → Term.Rewritable t₁ t₂ t₃' t₄' → Formula.Rewritable t₁ t₂ (t₁' ≈ t₃') (t₂' ≈ (t₄' : Term 𝓛)) :=
---   λ h₁ h₂ => atom (Terms.Rewritable.cons h₁ (Terms.Rewritable.cons h₂ Terms.Rewritable.nil))
-
--- def not : Formula.Rewritable t₁ t₂ p₁ p₂ → Formula.Rewritable t₁ t₂ (~ p₁) (~ p₂) :=
---   λ h => imp h fal
-
--- def or : Formula.Rewritable t₁ t₂ p₁ p₂ → Formula.Rewritable t₁ t₂ q₁ q₂ → Formula.Rewritable t₁ t₂ (p₁ ⋁ q₁) (p₂ ⋁ q₂) :=
---   λ h₁ h₂ => imp (not h₁) h₂
-
--- def and : Formula.Rewritable t₁ t₂ p₁ p₂ → Formula.Rewritable t₁ t₂ q₁ q₂ → Formula.Rewritable t₁ t₂ (p₁ ⋀ q₁) (p₂ ⋀ q₂) :=
---   λ h₁ h₂ => not (imp h₁ (not h₂))
-
--- def iff : Formula.Rewritable t₁ t₂ p₁ p₂ → Formula.Rewritable t₁ t₂ q₁ q₂ → Formula.Rewritable t₁ t₂ (p₁ ⟷ q₁) (p₂ ⟷ q₂) :=
---   λ h₁ h₂ => and (imp h₁ h₂) (imp h₂ h₁)
-
--- end Formula.Rewritable
+inductive Formula.Rewritable (Γ : Context 𝓛) : Formula 𝓛 → Formula 𝓛 → Prop where
+| atom : Terms.Rewritable Γ ts₁ ts₂ → Formula.Rewritable Γ (p ⬝ₚ ts₁) (p ⬝ₚ ts₂)
+| imp : Formula.Rewritable Γ p₁ p₂ → Formula.Rewritable Γ q₁ q₂ →
+  Formula.Rewritable Γ (p₁ ⟶ q₁) (p₂ ⟶ q₂)
+| refl : Formula.Rewritable Γ p p
 
 mutual
-theorem Term.Rewritable.soundness {Γ : Context 𝓛} {t₁' : Term 𝓛} :
-  Γ ⊢ t₁ ≈ t₂ → 𝓣.toContext ⊆ Γ → Term.Rewritable t₁ t₂ t₁' t₂' →
-  Γ ⊢ t₁' ≈ t₂' := λ h₁ h₂ h =>
-  match h with
-  | Term.Rewritable.matched => h₁
-  | Term.Rewritable.refl => Proof.weaken h₂ Proof.refl
-  | Term.Rewritable.func h => Proof.mp (Proof.weaken h₂ Proof.congr_func) (Terms.Rewritable.soundness h₁ h₂ h)
-theorem Terms.Rewritable.soundness {Γ : Context 𝓛} {ts₁ : Terms 𝓛 n} :
-  Γ ⊢ t₁ ≈ t₂ → 𝓣.toContext ⊆ Γ → Terms.Rewritable t₁ t₂ ts₁ ts₂ →
-  Γ ⊢ ts₁ ≋ ts₂ := λ h₁ h₂ h =>
-  match h with
-  | Terms.Rewritable.nil => Proof.true_intro
-  | Terms.Rewritable.cons h h' => Proof.mp2 Proof.and_intro (Term.Rewritable.soundness h₁ h₂ h) (Terms.Rewritable.soundness h₁ h₂ h')
+theorem Term.Rewritable.soundness (h : 𝓣.toContext ⊆ Γ) : Term.Rewritable Γ t₁ t₂ → Γ ⊢ t₁ ≈ t₂
+| Term.Rewritable.matched h₁ => h₁
+| Term.Rewritable.refl => Proof.weaken h Proof.refl
+| Term.Rewritable.func h₁ => Proof.mp (Proof.weaken h Proof.congr_func) (Terms.Rewritable.soundness h h₁)
+theorem Terms.Rewritable.soundness (h : 𝓣.toContext ⊆ Γ) : Terms.Rewritable Γ ts₁ ts₂ → Γ ⊢ ts₁ ≋ ts₂
+| Terms.Rewritable.nil => Proof.true_intro
+| Terms.Rewritable.cons h₁ h₂ => Proof.mp2 Proof.and_intro (Term.Rewritable.soundness h h₁) (Terms.Rewritable.soundness h h₂)
 end
 
-theorem Formula.Rewritable.soundness {Γ : Context 𝓛} :
-  𝓣.toContext ⊆ Γ → Γ ⊢ t₁ ≈ t₂ → Formula.Rewritable t₁ t₂ p₁ p₂ →
-  Γ ⊢ p₁ ⟷ p₂ := by
-  intros h₂ h₁ h
-  induction h with
-  | atom h => 
-    apply Proof.mp
-    · exact Proof.weaken h₂ Proof.congr_atom_iff
-    · exact Terms.Rewritable.soundness h₁ h₂ h
-  | fal => exact Proof.iff_refl
-  | imp _ _ ih₁ ih₂ =>
-    apply Proof.mp2 Proof.iff_congr_imp <;> assumption
-  | all => exact Proof.iff_refl
+theorem Formula.Rewritable.soundness (h : 𝓣.toContext ⊆ Γ) :
+  Formula.Rewritable Γ p q → Γ ⊢ p ⟷ q
+| Formula.Rewritable.atom h₁ => Proof.mp (Proof.weaken h Proof.congr_atom_iff) (Terms.Rewritable.soundness h h₁)
+| Formula.Rewritable.imp h₁ h₂ => Proof.mp2 Proof.iff_congr_imp (Formula.Rewritable.soundness h h₁) (Formula.Rewritable.soundness h h₂)
+| Formula.Rewritable.refl => Proof.iff_refl
 
-macro "prw" "by" t:tactic : tactic => `(tactic| (
-    apply Proof.mp2 Proof.iff_right
-    · apply Formula.Rewritable.soundness (by pweaken_ctx)
-      · ($t; skip)
-      · focus repeat' constructor
-    simp
-  ))
+macro "prw_by" t:tactic : tactic => `(tactic| (
+  apply Proof.mp2 Proof.iff_right
+  · apply Formula.Rewritable.soundness (by pweaken_ctx)
+    focus repeat' (
+      first
+      | exact Term.Rewritable.matched (by ($t; skip))
+      | eapply Formula.Rewritable.atom
+      | eapply Formula.Rewritable.imp
+      | exact Terms.Rewritable.nil
+      | eapply Terms.Rewritable.cons
+      | eapply Term.Rewritable.func
+      | exact Formula.Rewritable.refl
+      | exact Term.Rewritable.refl)
+  simp))
 
-macro "prw" t:term : tactic => `(tactic| prw by exact $t)
-macro "prw" "←" t:term : tactic => `(tactic| prw by (psymm; exact $t))
-macro "prww" t:term : tactic => `(tactic| prw by (apply Proof.weaken _ $t; pweaken_ctx))
-macro "prww" "←" t:term : tactic => `(tactic| prw by (psymm; apply Proof.weaken _ $t; pweaken_ctx))
-macro "prw" n:num : tactic => `(tactic| prw by passumption $n)
-macro "prw" "←" n:num : tactic => `(tactic| prw by (psymm; passumption $n))
+syntax "prwa" "←"? num : tactic
+macro_rules
+| `(tactic| prwa $n) => `(tactic| prw_by passumption $n)
+| `(tactic| prwa ←$n) => `(tactic| prw_by (psymm; passumption $n))
+
+syntax "prw" "←"? term : tactic
+macro_rules
+| `(tactic| prw $t) =>
+  `(tactic| prw_by (exact Proof.weaken (by pweaken_ctx) $t))
+| `(tactic| prw ←$t) =>
+  `(tactic| prw_by (psymm; exact Proof.weaken (by pweaken_ctx) $t))
